Add join_op_upperbound_right as corollary

Classes/Joinable.v
@@ -6,11 +6,17 @@ Class Joinable (T : Type) `{T_preorder : PreorderedSet T} : Type :=
   join_op : T -> T -> T;
   join_idem : ∀ x, join_op x x = x;
   join_upper_bound_left: forall t t', preorder t (join_op t t');
-  join_upper_bound_right: forall t t', preorder t' (join_op t t');
   join_assoc : ∀ x y z : T, 
     join_op x (join_op y z) = join_op (join_op x y) z;
   join_comm : ∀ x y, join_op x y = join_op y x;
 }.
+
+Corollary join_upper_bound_right {T : Type} `{Joinable T} : ∀ t t',
+  preorder t' (join_op t t').
+Proof.
+  intros. rewrite join_comm. apply join_upper_bound_left.
+Qed.
+
 Arguments join_op : simpl never.
 Hint Resolve join_upper_bound_left join_upper_bound_right : soundness.
 Hint Rewrite @join_idem : soundness.
